Worklist_Algorithms/Liveness_Subsumption_Map.thy
@@ -2,8 +2,8 @@ theory Liveness_Subsumption_Map
   imports Liveness_Subsumption "../library/DRAT_Misc"
 begin
 
-locale Search_Space_Nodes_Empty_Key_Defs =
-  Search_Space_Nodes_Empty_Defs E for E :: "'v \<Rightarrow> 'v \<Rightarrow> bool" +
+locale Liveness_Search_Space_Key_Defs =
+  Liveness_Search_Space_Defs E for E :: "'v \<Rightarrow> 'v \<Rightarrow> bool" +
   fixes key :: "'v \<Rightarrow> 'k"
 begin
 
@@ -13,42 +13,46 @@ definition "insert_map_set v S \<equiv>
   let k = key v; S' = (case S k of Some S \<Rightarrow> S | None \<Rightarrow> {}) in S(k \<mapsto> (insert v S'))
 "
 
-definition "check_subsumption v S \<equiv>
+definition "push_map_list v S \<equiv>
+  let k = key v; S' = (case S k of Some S \<Rightarrow> S | None \<Rightarrow> []) in S(k \<mapsto> v # S')
+"
+
+definition "check_subsumption_map_set v S \<equiv>
   let k = key v; S' = (case S k of Some S \<Rightarrow> S | None \<Rightarrow> {}) in (\<exists> x \<in> S'. v \<preceq> x)
 "
 
-definition "check_subsumption' v S \<equiv>
-  let k = key v; S' = (case S k of Some S \<Rightarrow> S | None \<Rightarrow> {}) in (\<exists> x \<in> S'. x \<preceq> v)
+definition "check_subsumption_map_list v S \<equiv>
+  let k = key v; S' = (case S k of Some S \<Rightarrow> S | None \<Rightarrow> []) in (\<exists> x \<in> set S'. x \<preceq> v)
 "
 
-definition "delete_map_set v S \<equiv>
-  let k = key v; S' = (case S k of Some S \<Rightarrow> S | None \<Rightarrow> {}) in S(k \<mapsto> (S' - {v}))
+definition "pop_map_list v S \<equiv>
+  let k = key v; S' = (case S k of Some S \<Rightarrow> tl S | None \<Rightarrow> []) in S(k \<mapsto> S')
 "
 
 definition dfs_map :: "('k \<rightharpoonup> 'v set) \<Rightarrow> (bool \<times> ('k \<rightharpoonup> 'v set)) nres" where
   "dfs_map P \<equiv> do {
     (P,ST,r) \<leftarrow> RECT (\<lambda>dfs (P,ST,v).
-      if check_subsumption' v ST then RETURN (P, ST, True)
+      if check_subsumption_map_list v ST then RETURN (P, ST, True)
       else do {
-        if check_subsumption v P then
+        if check_subsumption_map_set v P then
           RETURN (P, ST, False)
         else do {
-            let ST = insert_map_set v ST;
+            let ST = push_map_list v ST;
             (P, ST, r) \<leftarrow>
-              FOREACH\<^sub>C {v' . v \<rightarrow> v'} (\<lambda>(_,_,b). \<not>b) (\<lambda>v' (P,ST,_). dfs (P,ST,v')) (P,ST,False);
-            let ST = delete_map_set v ST;
+              nfoldli (succs v) (\<lambda>(_,_,b). \<not>b) (\<lambda>v' (P,ST,_). dfs (P,ST,v')) (P,ST,False);
+            let ST = pop_map_list v ST;
             let P = insert_map_set v P;
             RETURN (P, ST, r)
           }
       }
-    ) (P,Map.empty,a\<^sub>0);
+    ) (P,(Map.empty::('k \<rightharpoonup> 'v list)),a\<^sub>0);
     RETURN (r, P)
   }"
 
 end (* Search Space Nodes Empty Key Defs *)
 
-locale Search_Space_Nodes_finite_strict_Key =
-  Search_Space_Nodes_finite_strict + Search_Space_Nodes_Empty_Key_Defs +
+locale Liveness_Search_Space_Key =
+  Liveness_Search_Space + Liveness_Search_Space_Key_Defs +
   assumes subsumes_key[intro, simp]: "a \<preceq> b \<Longrightarrow> key a = key b"
 begin
 
@@ -57,20 +61,29 @@ definition
   "map_set_rel =
     {(m, s). \<Union> ran m = s \<and> (\<forall> k. \<forall> x. m k = Some x \<longrightarrow> (\<forall> v \<in> x. key v = k))}"
 
+term sorted
+
+definition
+  "map_list_rel =
+    {(m, xs). \<Union> (set ` ran m) = set xs \<and> (\<forall> k. \<forall> x. m k = Some x \<longrightarrow> (\<forall> v \<in> set x. key v = k))
+          \<and> (\<exists> R. (\<forall> k. \<forall> x. m k = Some x \<longrightarrow> sorted_by_rel R x) \<and> sorted_by_rel R xs)
+          \<and> distinct xs
+    }"
+
 definition "list_set_rel \<equiv> {(l, s). set l = s \<and> distinct l}"
 
 definition "list_set_hd_rel x \<equiv> {(l, s). set l = s \<and> distinct l \<and> l \<noteq> [] \<and> hd l = x}"
 
-lemma rel_start[refine]:
-  "((P, Map.empty, a\<^sub>0), P', {}, a\<^sub>0) \<in> map_set_rel \<times>\<^sub>r map_set_rel \<times>\<^sub>r Id" if "(P, P') \<in> map_set_rel"
-  using that unfolding map_set_rel_def list_set_rel_def by auto
+lemma
+  "(Map.empty, []) \<in> map_list_rel"
+  unfolding map_list_rel_def by auto
 
-lemma check_loop_ref[refine]:
-  "check_loop_list x xs = check_loop x S" if "(xs, S) \<in> list_set_rel"
-  using that unfolding check_loop_list_def check_loop_def list_set_rel_def by auto
+lemma rel_start[refine]:
+  "((P, Map.empty, a\<^sub>0), P', [], a\<^sub>0) \<in> map_set_rel \<times>\<^sub>r map_list_rel \<times>\<^sub>r Id" if "(P, P') \<in> map_set_rel"
+  using that unfolding map_set_rel_def map_list_rel_def by auto
 
 lemma refine_True:
-  "(x1b, x1) \<in> map_set_rel \<Longrightarrow> (x1c, x1a) \<in> map_set_rel \<Longrightarrow> ((x1b, x1c, True), x1, x1a, True) \<in> map_set_rel \<times>\<^sub>r map_set_rel \<times>\<^sub>r Id"
+  "(x1b, x1) \<in> map_set_rel \<Longrightarrow> (x1c, x1a) \<in> map_list_rel \<Longrightarrow> ((x1b, x1c, True), x1, x1a, True) \<in> map_set_rel \<times>\<^sub>r map_list_rel \<times>\<^sub>r Id"
   by simp
 
 lemma refine_True':
@@ -78,14 +91,19 @@ lemma refine_True':
   unfolding map_set_rel_def list_set_rel_def oops
 
 lemma check_subsumption_ref[refine]:
-  "(x1b, x1) \<in> map_set_rel \<Longrightarrow> check_subsumption x2a x1b = (\<exists>x\<in>x1. x2a \<preceq> x)"
-  unfolding map_set_rel_def list_set_rel_def check_subsumption_def
+  "(x1b, x1) \<in> map_set_rel \<Longrightarrow> check_subsumption_map_set x2a x1b = (\<exists>x\<in>x1. x2a \<preceq> x)"
+  unfolding map_set_rel_def list_set_rel_def check_subsumption_map_set_def
   unfolding ran_def by (auto split: option.splits)
 
 lemma check_subsumption'_ref[refine]:
-  "(x1b, x1) \<in> map_set_rel \<Longrightarrow> check_subsumption' x2a x1b = check_loop x2a x1"
-  unfolding map_set_rel_def list_set_rel_def check_subsumption'_def check_loop_def
-  unfolding ran_def by (force split: option.splits)
+  "(m, xs) \<in> map_list_rel \<Longrightarrow> check_subsumption_map_list x m = check_loop x xs"
+  unfolding map_list_rel_def list_set_rel_def check_subsumption_map_list_def check_loop_def
+  unfolding ran_def apply (auto split: option.splits)
+  subgoal for R x' xs'
+    apply rule
+     apply assumption
+    sorry
+  by force
 
 lemma not_check_loop_non_elem:
   "x \<notin> set xs" if "\<not> check_loop_list x xs"
@@ -99,8 +117,7 @@ lemma insert_ref[refine]:
   unfolding list_set_hd_rel_def list_set_rel_def by (auto dest: not_check_loop_non_elem)
 
 lemma insert_map_set_ref:
-  "(m, S) \<in> map_set_rel \<Longrightarrow>
-   (insert_map_set x m, insert x S) \<in> map_set_rel"
+  "(m, S) \<in> map_set_rel \<Longrightarrow> (insert_map_set x m, insert x S) \<in> map_set_rel"
   unfolding insert_map_set_def insert_def map_set_rel_def
   apply (auto split: option.splits)
   subgoal for x' S'
@@ -119,6 +136,94 @@ lemma insert_map_set_ref:
     unfolding ran_def Let_def by (auto split: option.splits if_split_asm)
   done
 
+lemma map_list_rel_memD:
+  assumes "(m, xs) \<in> map_list_rel" "x \<in> set xs"
+  obtains xs' where "x \<in> set xs'" "m (key x) = Some xs'"
+  apply atomize_elim
+  using assms
+  unfolding map_list_rel_def
+  apply auto
+  unfolding ran_def
+    sorry
+
+lemma map_list_rel_memI:
+  "(m, xs) \<in> map_list_rel \<Longrightarrow> m k = Some xs' \<Longrightarrow> x' \<in> set xs' \<Longrightarrow> x' \<in> set xs"
+  unfolding map_list_rel_def ran_def by auto
+
+lemma map_list_rel_grouped_by_key:
+  "x' \<in> set xs' \<Longrightarrow> (m, xs) \<in> map_list_rel \<Longrightarrow> m k = Some xs' \<Longrightarrow> key x' = k"
+  unfolding map_list_rel_def by auto
+
+lemma map_list_rel_not_memI:
+  "k \<noteq> key x \<Longrightarrow> m k = Some xs' \<Longrightarrow> (m, xs) \<in> map_list_rel \<Longrightarrow> x \<notin> set xs'"
+  unfolding map_list_rel_def by auto
+
+lemma map_list_rel_not_memI2:
+  "x \<notin> set xs'" if "m a = Some xs'" "(m, xs) \<in> map_list_rel" "x \<notin> set xs"
+  using that unfolding map_list_rel_def ran_def by auto
+
+lemma push_map_list_ref:
+  "x \<notin> set xs \<Longrightarrow> (m, xs) \<in> map_list_rel \<Longrightarrow> (push_map_list x m, x # xs) \<in> map_list_rel"
+  unfolding push_map_list_def
+  apply (subst map_list_rel_def)
+  apply auto
+  subgoal for x' xs'
+    unfolding ran_def Let_def
+     by (auto split: option.split_asm if_split_asm intro: map_list_rel_memI)
+  subgoal
+    unfolding ran_def Let_def by (auto 4 3 split: option.splits if_splits)
+  subgoal for x'
+    unfolding ran_def Let_def
+    apply (erule map_list_rel_memD, assumption)
+      apply (cases "key x = key x'")
+    subgoal for xs'
+      by auto
+        subgoal for xs'
+      apply (rule bexI[where x = xs'])
+           apply safe
+      apply (inst_existentials "key x'")
+          apply force
+          done
+        done
+      subgoal for k xs' x'
+        unfolding Let_def
+        by (auto split: option.split_asm if_split_asm dest: map_list_rel_grouped_by_key)
+      subgoal
+      proof -
+        assume A: "x \<notin> set xs" "(m, xs) \<in> map_list_rel"
+        then obtain R where *:
+          "x \<notin> set xs"
+          "UNION (ran m) set = set xs"
+          "\<forall>k x. m k = Some x \<longrightarrow> (\<forall>v\<in>set x. key v = k)"
+          "distinct xs"
+          "\<forall>k x. m k = Some x \<longrightarrow> sorted_by_rel R x"
+          "sorted_by_rel R xs"
+          unfolding map_list_rel_def by auto
+        have **: "sorted_by_rel (\<lambda>a b. a = x \<or> R a b) xs" if
+          "sorted_by_rel R xs" "x \<notin> set xs" for xs
+          using that by (induction xs) auto
+
+        show ?thesis
+          apply (inst_existentials "\<lambda> a b. a = x \<or> R a b")
+              apply auto
+            unfolding Let_def
+             apply (auto split: option.split_asm if_split_asm)
+            subgoal for k xs'
+              apply (drule map_list_rel_not_memI, assumption, rule A)
+              using *(5)
+              by (auto intro: **)
+            subgoal for xs'
+              using A(1) *(5)
+              by (auto intro: ** A dest: map_list_rel_not_memI2)
+            subgoal for xs'
+              using A(1) *(5)
+              by (auto 4 3 intro: ** A dest: map_list_rel_not_memI2)
+            subgoal
+              using A by (auto intro: * **)
+            done
+        qed
+        by (auto simp: map_list_rel_def)
+
 lemma insert_map_set_ref'[refine]:
   "(x1b, x1) \<in> map_set_rel \<Longrightarrow>
    (x1c, x1a) \<in> map_set_rel \<Longrightarrow>
@@ -126,8 +231,15 @@ lemma insert_map_set_ref'[refine]:
    ((x1b, insert_map_set x2a x1c, False), x1, insert x2a x1a, False) \<in> map_set_rel \<times>\<^sub>r map_set_rel \<times>\<^sub>r Id"
   by (auto intro: insert_map_set_ref)
 
-lemma delete_map_set_ref[refine]:
-  "(delete_map_set x m, S - {x}) \<in> map_set_rel" if "(m, S) \<in> map_set_rel"
+lemma push_map_list_ref'[refine]:
+  "(x1b, x1) \<in> map_set_rel \<Longrightarrow>
+   (x1c, x1a) \<in> map_list_rel \<Longrightarrow>
+   \<not> check_subsumption_map_list x2a x1c \<Longrightarrow>
+   ((x1b, push_map_list x2a x1c, False), x1, x2a # x1a, False) \<in> map_set_rel \<times>\<^sub>r map_list_rel \<times>\<^sub>r Id"
+  by (auto intro: push_map_list_ref)
+
+lemma pop_map_list_ref[refine]:
+  "(pop_map_list v m, tl S) \<in> map_list_rel" if "(m, S) \<in> map_list_rel"
   using that unfolding map_set_rel_def delete_map_set_def
   apply (auto split: option.splits if_split_asm simp: Let_def)
   subgoal for X
@@ -142,6 +254,8 @@ lemma delete_map_set_ref[refine]:
     by (metis insertE insert_Diff option.inject set_minus_singleton_eq)
   done
 
+thm pop_map_list_ref
+
 lemma tl_list_set_ref:
   "(m, S) \<in> map_set_rel \<Longrightarrow>
    (st, ST) \<in> list_set_hd_rel x \<Longrightarrow>
@@ -152,6 +266,10 @@ lemma tl_list_set_ref:
   apply (simp add: distinct_hd_tl)
   by (meson in_hd_or_tl_conv)
 
+lemma succs_id_ref:
+  "(succs x, succs x) \<in> \<langle>Id\<rangle> list_rel"
+  by simp
+
 lemma dfs_map_dfs_refine:
   "dfs_map P \<le> \<Down> (Id \<times>\<^sub>r map_set_rel) (dfs P')" if "(P, P') \<in> map_set_rel"
   using that
@@ -161,34 +279,32 @@ lemma dfs_map_dfs_refine:
             apply (clarsimp, rule check_subsumption'_ref, assumption)
            apply (clarsimp, rule refine_True; assumption)
           apply (clarsimp, rule check_subsumption_ref; assumption)
-         apply (simp; fail)
-        apply (rule inj_on_id; fail)
-         apply (simp; fail)
-      apply (clarsimp, rule insert_map_set_ref'; assumption)
-      by (auto intro: insert_map_set_ref delete_map_set_ref)
+          apply (simp; fail)
+         apply (clarsimp; rule succs_id_ref; fail)
+      apply (clarsimp, rule push_map_list_ref'; assumption)
+      by (auto intro: insert_map_set_ref pop_map_list_ref)
 
 end (* Search Space Nodes Finite Strict Key *)
 
-locale Search_Space_Nodes_Empty_Key1_Defs =
-  Search_Space_Nodes_Empty_Key_Defs +
+(*
+locale Liveness_Search_Space_Key1_Defs =
+  Liveness_Search_Space_Key_Defs +
   fixes succs :: "'a \<Rightarrow> 'a list"
 begin
-
-term succs
 
 definition dfs_map1 :: "('b \<rightharpoonup> 'a set) \<Rightarrow> (bool \<times> ('b \<rightharpoonup> 'a set)) nres" where
   "dfs_map1 P \<equiv> do {
     (P,ST,r) \<leftarrow> RECT (\<lambda>dfs (P,ST,v).
-      if check_subsumption' v ST then RETURN (P, ST, True)
+      if check_subsumption_map_list v ST then RETURN (P, ST, True)
       else do {
-        if check_subsumption v P then
+        if check_subsumption_map_set v P then
           RETURN (P, ST, False)
         else do {
-            let ST = insert_map_set v ST;
+            let ST = push_map_list v ST;
             ASSERT (reachable v);
             (P, ST, r) \<leftarrow>
               FOREACH\<^sub>C (set (succs v)) (\<lambda>(_,_,b). \<not>b) (\<lambda>v' (P,ST,_). dfs (P,ST,v')) (P,ST,False);
-            let ST = delete_map_set v ST;
+            let ST = pop_map_list v ST;
             let P = insert_map_set v P;
             RETURN (P, ST, r)
           }
@@ -221,5 +337,6 @@ lemma
   by (auto 4 3 dest: reachable_step succs_correct) (* XXX Add to automation? *)
 
 end (* Search Space Nodes Finite Strict Key 1 *)
+*)
 
 end (* Theory *)
