Worklist_Algorithms/Liveness_Subsumption_Impl.thy
@@ -1,0 +1,199 @@
+theory Liveness_Subsumption_Impl
+  imports Liveness_Subsumption_Map Heap_Hash_Map
+begin
+
+locale Liveness_Search_Space_Key_Impl_Defs =
+  Liveness_Search_Space_Key_Defs _ _ _ _ _ _ _ key for key :: "'a \<Rightarrow> 'ki :: {hashable, heap}" +
+  fixes A :: "'a \<Rightarrow> ('ai :: heap) \<Rightarrow> assn"
+  fixes succsi :: "'ai \<Rightarrow> 'ai list Heap"
+  fixes a\<^sub>0i :: "'ai Heap"
+  fixes Lei :: "'ai \<Rightarrow> 'ai \<Rightarrow> bool Heap"
+  fixes keyi :: "'ai \<Rightarrow> 'ki Heap"
+  fixes copyi :: "'ai \<Rightarrow> 'ai Heap"
+
+locale Liveness_Search_Space_Key_Impl =
+  Liveness_Search_Space_Key_Impl_Defs +
+  Liveness_Search_Space_Key +
+  assumes [sepref_fr_rules]: "(uncurry0 a\<^sub>0i, uncurry0 (RETURN (PR_CONST a\<^sub>0))) \<in> unit_assn\<^sup>k \<rightarrow>\<^sub>a A"
+  assumes [sepref_fr_rules]: "(Fi,RETURN o PR_CONST F') \<in> A\<^sup>k \<rightarrow>\<^sub>a bool_assn"
+  assumes [sepref_fr_rules]: "(uncurry Lei,uncurry (RETURN oo PR_CONST op \<preceq>)) \<in> A\<^sup>k *\<^sub>a A\<^sup>k \<rightarrow>\<^sub>a bool_assn"
+  assumes [sepref_fr_rules]: "(succsi,RETURN o PR_CONST succs) \<in> A\<^sup>k \<rightarrow>\<^sub>a list_assn A"
+  assumes [sepref_fr_rules]: "(keyi,RETURN o PR_CONST key) \<in> A\<^sup>k \<rightarrow>\<^sub>a id_assn"
+  assumes [sepref_fr_rules]: "(copyi, RETURN o COPY) \<in> A\<^sup>k \<rightarrow>\<^sub>a A"
+
+
+context Liveness_Search_Space_Key_Impl_Defs
+begin
+
+(* XXX The lemma has this form to avoid unwanted eta-expansions.
+  The eta-expansions arise from the type of 'insert_map_set v S' *)
+lemma insert_map_set_alt_def: "(None, insert_map_set v S) = (
+  let
+    k = key v; (S', S) = op_map_extract k S
+  in
+    case S' of
+      Some S1 \<Rightarrow> (None, S(k \<mapsto> (insert v S1)))
+    | None \<Rightarrow> (None, S(k \<mapsto> {v}))
+)
+"
+  unfolding insert_map_set_def op_map_extract_def by (auto simp: Let_def split: option.split)
+
+lemma check_subsumption_map_set_alt_def: "check_subsumption_map_set v S = (
+  let
+    k = key v; (S', S) = op_map_extract k S;
+    S1' = (case S' of Some S1 \<Rightarrow> S1 | None \<Rightarrow> {})
+  in (\<exists> x \<in> S1'. v \<preceq> x)
+)
+"
+  unfolding check_subsumption_map_set_def op_map_extract_def by (auto simp: Let_def)
+
+lemma check_subsumption_map_set_extract: "(S, check_subsumption_map_set v S) = (
+  let
+    k = key v; (S', S) = op_map_extract k S
+  in (
+    case S' of
+      Some S1 \<Rightarrow> (let r = (\<exists> x \<in> S1. v \<preceq> x) in (op_map_update k S1 S, r))
+    | None \<Rightarrow> (S, False)
+  )
+)
+"
+  unfolding check_subsumption_map_set_def op_map_extract_def op_map_update_def op_map_delete_def
+  by (auto simp: Let_def split: option.split)
+
+lemma check_subsumption_map_list_extract: "(S, check_subsumption_map_list v S) = (
+  let
+    k = key v; (S', S) = op_map_extract k S
+  in (
+    case S' of
+      Some S1 \<Rightarrow> (let r = (\<exists> x \<in> set S1. x \<preceq> v) in (op_map_update k S1 S, r))
+    | None \<Rightarrow> (S, False)
+  )
+)
+"
+  unfolding check_subsumption_map_list_def op_map_extract_def op_map_update_def op_map_delete_def
+  by (auto simp: Let_def split: option.split)
+
+lemma push_map_list_alt_def: "(None, push_map_list v S) = (
+  let
+    k = key v; (S', S) = op_map_extract k S
+  in
+    case S' of
+      Some S1 \<Rightarrow> (None, S(k \<mapsto> v # S1))
+    | None \<Rightarrow> (None, S(k \<mapsto> [v]))
+)
+"
+  unfolding push_map_list_def op_map_extract_def by (auto simp: Let_def split: option.split)
+
+(* XXX The check for emptiness is superfluous if we thread through the pre-condition *)
+lemma pop_map_list_alt_def: "(None, pop_map_list v S) = (
+  let
+    k = key v; (S', S) = op_map_extract k S
+  in
+    case S' of
+      Some S1 \<Rightarrow> (None, S(k \<mapsto> if op_list_is_empty S1 then [] else tl S1))
+    | None \<Rightarrow> (None, S(k \<mapsto> []))
+)
+"
+  unfolding pop_map_list_def op_map_extract_def by (auto simp: Let_def split: option.split)
+
+lemmas alt_defs =
+  insert_map_set_alt_def check_subsumption_map_set_extract
+  check_subsumption_map_list_extract pop_map_list_alt_def push_map_list_alt_def
+
+lemma dfs_map_alt_def:
+  "dfs_map P = do {
+    (P,ST,r) \<leftarrow> RECT (\<lambda>dfs (P,ST,v).
+      let (ST, b) = (ST, check_subsumption_map_list v ST) in
+      if b then RETURN (P, ST, True)
+      else do {
+        let (P, b1) = (P, check_subsumption_map_set v P) in
+        if b1 then
+          RETURN (P, ST, False)
+        else do {
+            let (_, ST1) = (None, push_map_list (COPY v) ST);
+            (P1, ST2, r) \<leftarrow>
+              nfoldli (succs v) (\<lambda>(_,_,b). \<not>b) (\<lambda>v' (P,ST,_). dfs (P,ST,v')) (P,ST1,False);
+            let (_, ST') = (None, pop_map_list (COPY v) ST2);
+            let (_, P') = (None, insert_map_set (COPY v) P1);
+            RETURN (P', ST', r)
+          }
+      }
+    ) (P,Map.empty,a\<^sub>0);
+    RETURN (r, P)
+  }"
+  unfolding dfs_map_def
+  unfolding Let_def
+  unfolding COPY_def
+  by auto
+
+end (* Search Space Nodes Empty Key Impl Defs 1 *)
+
+definition (in imp_map_delete) [code_unfold]: "hms_delete = delete"
+
+lemma (in imp_map_delete) hms_delete_rule [sep_heap_rules]:
+  "<hms_assn A m mi> hms_delete k mi <hms_assn A (m(k := None))>\<^sub>t"
+  unfolding hms_delete_def hms_assn_def
+  apply (sep_auto eintros del: exI)
+  subgoal for mh
+    apply (rule exI[where x = "mh(k := None)"])
+    apply (rule ent_frame_fwd[OF map_assn_delete[where A = A]], frame_inference)
+    by sep_auto
+  done
+
+context imp_map_delete
+begin
+
+lemma hms_delete_hnr:
+  "(uncurry hms_delete, uncurry (RETURN oo op_map_delete)) \<in>
+  id_assn\<^sup>k *\<^sub>a (hms_assn A)\<^sup>d \<rightarrow>\<^sub>a hms_assn A"
+  by sepref_to_hoare sep_auto
+
+sepref_decl_impl delete: hms_delete_hnr uses op_map_delete.fref[where V = Id] .
+
+end
+
+lemma fold_insert_set:
+  "fold insert xs S = set xs \<union> S"
+  by (induction xs arbitrary: S) auto
+
+lemma set_alt_def:
+  "set xs = fold insert xs {}"
+  by (simp add: fold_insert_set)
+
+(* XXX Duplication *)
+lemma list_ex_foldli:
+  "list_ex P xs = foldli xs Not (\<lambda> x y. P x \<or> y) False"
+ apply (induction xs)
+ apply (simp; fail)
+ subgoal for x xs
+  apply simp
+  apply (induction xs)
+ by auto
+ done
+
+context Liveness_Search_Space_Key_Impl
+begin
+
+sepref_register
+  "PR_CONST a\<^sub>0" "PR_CONST op \<preceq>" "PR_CONST succs" "PR_CONST key"
+
+lemma [def_pat_rules]:
+  "a\<^sub>0 \<equiv> UNPROTECT a\<^sub>0" "op \<preceq> \<equiv> UNPROTECT op \<preceq>" "succs \<equiv> UNPROTECT succs"
+  "keyi \<equiv> UNPROTECT keyi" "key \<equiv> UNPROTECT key"
+  by simp_all
+
+(* lemma [safe_constraint_rules]: "CN_FALSE is_pure A \<Longrightarrow> is_pure A" by simp *)
+
+sepref_thm dfs_map1_impl is
+  "uncurry0 (do {(r, p) \<leftarrow> dfs_map Map.empty; RETURN r})" :: "unit_assn\<^sup>k \<rightarrow>\<^sub>a bool_assn"
+  apply (subst dfs_map_alt_def)
+  unfolding alt_defs
+  unfolding Bex_set list_ex_foldli
+  unfolding fold_lso_bex
+  unfolding lso_fold_custom_empty hm.hms_fold_custom_empty HOL_list.fold_custom_empty
+  supply [[goals_limit = 1]]
+  by sepref
+
+end (* Search Space Nodes Finite Strict Key Impl 1 *)
+
+end (* Theory *)
